src/CCLMonadLaws.v
@@ -31,6 +31,17 @@ Section MonadLaws.
     - destruct out, st; eauto.
   Qed.
 
+  Theorem monad_debug_left_id : forall T' (p: _ -> cprog T') s,
+      exec_equiv (Bind (Debug s) p) (p tt).
+  Proof.
+    split; intros.
+    - inv_bind.
+      inv_debug; eauto.
+      inv_debug.
+    - eapply ExecBindFinish; eauto.
+      eapply ExecStepDec; eauto.
+  Qed.
+
   Theorem monad_assoc : forall T T' T''
                           (p1: cprog T)
                           (p2: T -> cprog T')
