src/CCLProg.v
@@ -120,6 +120,8 @@ Section CCL.
   | SetLock (l:LocalLock) (l':LocalLock) : cprog unit
   (* no-op to indicate interest in reading a *)
   | YieldTillReady (a:addr) : cprog unit
+  (* no-op for debugging *)
+  | Debug (s:String.string) : cprog unit
   | Ret T (v:T) : cprog T
   | Bind T T' (p: cprog T') (p': T' -> cprog T) : cprog T.
 
@@ -265,6 +267,7 @@ Section CCL.
                      else Fails (* caller didn't know its lock status *)
     | YieldTillReady _ => StepTo sigma tt
     | Ret v => StepTo sigma v
+    | Debug _ => StepTo sigma tt
     | _ => NonDet
     end.
 
@@ -445,6 +448,17 @@ Module CCLTactics.
       inversion H; subst; repeat inj_pair2;
       try match goal with
           | [ H: step_dec _ _ (Ret _) = _ |- _ ] =>
+            simpl in H; inversion H; subst; clear H
+          end;
+      clear H
+    end.
+
+  Ltac inv_debug :=
+    match goal with
+    | [ H: exec _ _ _ (Debug _) _ |- _ ] =>
+      inversion H; subst; repeat inj_pair2;
+      try match goal with
+          | [ H: step_dec _ _ (Debug _) = _ |- _ ] =>
             simpl in H; inversion H; subst; clear H
           end;
       clear H
